SMC wip

raft/proof/StateMachineCorrectProof.v
@@ -15,11 +15,236 @@ Local Arguments update {_} {_} {_} _ _ _ _ : simpl never.
 
 Require Import Raft.
 Require Import CommonDefinitions.
+Require Import CommonTheorems.
 
 Section StateMachineCorrect.
   Context {orig_base_params : BaseParams}.
   Context {one_node_params : OneNodeParams orig_base_params}.
   Context {raft_params : RaftParams orig_base_params}.
+
+  Ltac update_destruct :=
+    match goal with
+      | [ |- context [ update _ ?y _ ?x ] ] => destruct (name_eq_dec y x)
+    end.
+
+  Ltac update_destruct_hyp :=
+    match goal with
+      | [ _ : context [ update _ ?y _ ?x ] |- _ ] => destruct (name_eq_dec y x)
+    end.
+
+  Ltac destruct_update :=
+    repeat (first [update_destruct_hyp|update_destruct]; subst; rewrite_update).
+
+  Definition clientCache_to_ks (c : list (nat * (nat * output))) :=
+    map (fun e => (fst e, fst (snd e))) c.
+
+  Lemma snd_execute_log' :
+    forall l st o o',
+      snd (execute_log' l st o) = snd (execute_log' l st o').
+  Proof.
+    induction l; intros; simpl in *; intuition;
+    break_let; eauto.
+  Qed.
+
+
+  Lemma snd_execute_log'_nil :
+    forall l st o,
+      snd (execute_log' l st o) = snd (execute_log' l st []).
+  Proof.
+    eauto using snd_execute_log'.
+  Qed.
+  
+  Lemma clientCache_to_ks_assoc :
+    forall c client id,
+      assoc eq_nat_dec (clientCache_to_ks c) client = Some id ->
+      exists o,
+        assoc eq_nat_dec c client = Some (id, o).
+  Proof.
+    induction c; intros; simpl in *; try congruence.
+    break_if; eauto.
+    - subst. find_inversion.
+      break_let. subst. simpl in *. break_if; try congruence.
+      destruct p. simpl in *. eauto.
+    - break_let; subst; simpl in *. break_if; try congruence. eauto.
+  Qed.
+
+  Lemma clientCache_to_ks_assoc_getLastId :
+    forall st client id,
+      assoc eq_nat_dec (clientCache_to_ks (clientCache st)) client = Some id ->
+      exists o,
+        getLastId st client = Some (id, o).
+  Proof.
+    eauto using clientCache_to_ks_assoc.
+  Qed.
+
+  Lemma clientCache_to_ks_assoc_none :
+    forall c client,
+      assoc eq_nat_dec (clientCache_to_ks c) client = None ->
+      assoc eq_nat_dec c client = None.
+  Proof.
+    induction c; intros; simpl in *; try congruence.
+    break_if; eauto; try congruence.
+    - break_let; subst; simpl in *. break_if; try congruence. eauto.
+  Qed.
+
+  Lemma clientCache_to_ks_assoc_getLastId_none :
+    forall st client,
+      assoc eq_nat_dec (clientCache_to_ks (clientCache st)) client = None ->
+      getLastId st client = None.
+  Proof.
+    eauto using clientCache_to_ks_assoc_none.
+  Qed.
+  
+  Lemma cacheApplyEntry_stateMachine_apply :
+    forall st e os st' id o o' d,
+      cacheApplyEntry st e = (os, st') ->
+      getLastId st (eClient e) = Some (id, o) ->
+      id < eId e ->
+      handler (eInput e) (stateMachine st) = (o', d) ->
+      stateMachine st' = d.
+  Proof.
+    intros.
+    unfold cacheApplyEntry, applyEntry in *.
+    repeat break_match; subst; repeat find_inversion; do_bool; try omega;
+    simpl in *; auto.
+  Qed.
+
+  Lemma cacheApplyEntry_cache_apply :
+    forall st e os st' id o o' d,
+      cacheApplyEntry st e = (os, st') ->
+      getLastId st (eClient e) = Some (id, o) ->
+      id < eId e ->
+      handler (eInput e) (stateMachine st) = (o', d) ->
+      assoc_set eq_nat_dec (clientCache st) (eClient e) (eId e, o') = clientCache st'.
+  Proof.
+    intros.
+    unfold cacheApplyEntry, applyEntry in *.
+    repeat break_match; subst; repeat find_inversion; do_bool;
+    simpl in *; auto; omega.
+  Qed.
+
+
+  Lemma cacheApplyEntry_stateMachine_apply_none :
+    forall st e os st' o' d,
+      cacheApplyEntry st e = (os, st') ->
+      getLastId st (eClient e) = None ->
+      handler (eInput e) (stateMachine st) = (o', d) ->
+      stateMachine st' = d.
+  Proof.
+    intros.
+    unfold cacheApplyEntry, applyEntry in *.
+    repeat break_match; subst; repeat find_inversion; do_bool; try omega;
+    simpl in *; auto; congruence.
+  Qed.
+
+  Lemma cacheApplyEntry_cache_apply_none :
+    forall st e os st' o' d,
+      cacheApplyEntry st e = (os, st') ->
+      getLastId st (eClient e) = None ->
+      handler (eInput e) (stateMachine st) = (o', d) ->
+      assoc_set eq_nat_dec (clientCache st) (eClient e) (eId e, o') = clientCache st'.
+  Proof.
+    intros.
+    unfold cacheApplyEntry, applyEntry in *.
+    repeat break_match; subst; repeat find_inversion; do_bool;
+    simpl in *; auto; congruence.
+  Qed.
+
+  Lemma cacheApplyEntry_stateMachine_no_apply :
+    forall st e os st' id o,
+      cacheApplyEntry st e = (os, st') ->
+      getLastId st (eClient e) = Some (id, o) ->
+      eId e <= id ->
+      stateMachine st' = stateMachine st.
+  Proof.
+    intros.
+    unfold cacheApplyEntry, applyEntry in *.
+    repeat break_match; subst; repeat find_inversion; do_bool;
+    simpl in *; auto; try omega; congruence.
+  Qed.
+
+  Lemma cacheApplyEntry_cache_no_apply :
+    forall st e os st' id o,
+      cacheApplyEntry st e = (os, st') ->
+      getLastId st (eClient e) = Some (id, o) ->
+      eId e <= id ->
+      clientCache st = clientCache st'.
+  Proof.
+    intros.
+    unfold cacheApplyEntry, applyEntry in *.
+    repeat break_match; subst; repeat find_inversion; do_bool;
+    simpl in *; auto; try omega; congruence.
+  Qed.
+  
+  Lemma clientCache_to_ks_assoc_set :
+    forall c client id o,
+      assoc_set eq_nat_dec (clientCache_to_ks c) client id =
+      clientCache_to_ks (assoc_set eq_nat_dec c client (id, o)).
+  Proof.
+    induction c; intros; simpl in *; intuition.
+    simpl.
+    break_if; simpl in *; eauto.
+    f_equal. eauto.
+  Qed.
+  
+  Lemma applyEntries_execute_log' :
+    forall l h st os st',
+      applyEntries h st l = (os, st') ->
+      stateMachine st' = (snd (execute_log'
+                                 (deduplicate_log' l (clientCache_to_ks (clientCache st)))
+                                 (stateMachine st) [])).
+  Proof.
+    induction l; intros; simpl in *; intuition.
+    - find_inversion. auto.
+    - repeat break_let. find_inversion.
+      repeat break_match; simpl in *.
+      + break_let.
+        rewrite snd_execute_log'_nil.
+        find_apply_hyp_hyp. do_bool.
+        find_apply_lem_hyp clientCache_to_ks_assoc_getLastId.
+        break_exists.
+        find_copy_eapply_lem_hyp cacheApplyEntry_stateMachine_apply;
+          [|eauto|idtac|]; eauto. subst.
+        find_eapply_lem_hyp cacheApplyEntry_cache_apply; eauto.
+        erewrite clientCache_to_ks_assoc_set.
+        rewrite Heqp1. eauto.
+      + do_bool.
+        find_apply_hyp_hyp.
+        find_apply_lem_hyp clientCache_to_ks_assoc_getLastId.
+        break_exists.
+        break_exists.
+        find_copy_eapply_lem_hyp cacheApplyEntry_stateMachine_no_apply; eauto.
+        find_eapply_lem_hyp cacheApplyEntry_cache_no_apply; eauto.
+        repeat find_rewrite. auto.
+      + break_let. 
+        rewrite snd_execute_log'_nil.
+        find_apply_hyp_hyp. do_bool.
+        find_apply_lem_hyp clientCache_to_ks_assoc_getLastId_none.
+        break_exists.
+        find_copy_eapply_lem_hyp cacheApplyEntry_stateMachine_apply_none; eauto.
+        subst.
+        find_eapply_lem_hyp cacheApplyEntry_cache_apply_none; eauto.
+        erewrite clientCache_to_ks_assoc_set.
+        rewrite Heqp1. eauto.
+  Qed.
+  
+  Lemma state_machine_do_generic_server :
+    raft_net_invariant_do_generic_server state_machine_correct.
+  Proof.
+    red. unfold state_machine_correct. intros.
+    intuition.
+    - unfold state_machine_log in *. simpl in *. intros.
+      find_higher_order_rewrite.
+      destruct_update; simpl in *; eauto.
+      unfold doGenericServer in *. break_let.
+      find_inversion. simpl in *.
+      find_apply_lem_hyp applyEntries_execute_log'. repeat find_rewrite.
+      simpl in *. repeat find_higher_order_rewrite.
+      unfold client_cache_complete in *.
+      Lemma execute_log'_app :
+        forall l l' st os,
+          
+      
 
   Theorem state_machine_correct_invariant :
     forall net,
